different isBST causes timeout

fatnode/FatNode.dfy
@@ -1,45 +1,73 @@
-// class Entry {
-//   ghost var Repr: set<Node>
-//   ghost var ValueSets: seq<(int, set<int>)> 
+function {:opaque} VersionIndexHelper(version: int, versions: seq<int>, lo: int, hi: int): (index: int)
+  decreases hi - lo
+  requires |versions| == 0 ==> lo > hi && hi == -1
+  requires 0 <= lo <= |versions| 
+  requires -1 <= hi < |versions|
+  requires lo <= hi + 1
+  requires Sorted(versions)
+  requires forall k :: hi < k < |versions| ==> versions[k] > version
+  requires forall k :: 0 <= k < lo ==> versions[k] <= version
+  ensures -1 <= index < |versions|
+  ensures index == -1 <==> (|versions| == 0 || forall k :: 0 <= k < |versions| ==> versions[k] > version)
+  ensures index >= 0 <==> |versions| > 0 && versions[0] <= version
+  ensures index == -1 || versions[index] <= version
+  ensures forall i | 0 <= i < index :: versions[i] < version
+  ensures index >= 0 ==> forall i | index < i < |versions| :: versions[i] > version
+{
+  if (lo > hi) then
+    assert lo <= 0 || versions[lo - 1] <= version;
+    lo - 1
+  else
+    assert |versions| > 0;
+    var mid := lo + (hi - lo) / 2;
+    var v := versions[mid];
+    if v == version then
+      mid
+    else if v < version then
+      VersionIndexHelper(version, versions, mid + 1, hi)
+    else 
+      VersionIndexHelper(version, versions, lo, mid - 1)
+} 
 
-//   var roots: seq<Node?>
-//   var time: int
+function {:opaque} VersionIndex(version: int, versions: seq<int>): (index: int)
+  requires Sorted(versions)
+  ensures -1 <= index < |versions|
+  ensures index >= 0 <==> |versions| > 0 && versions[0] <= version
+  ensures index == -1 || IsMaxMinVersion(version, versions[index], versions)
+  ensures version in versions <==> index >= 0 && |versions| > index && versions[index] == version
+  ensures |versions| > 0 && version > versions[|versions| - 1] ==> index == |versions| - 1
+{
+  VersionIndexHelper(version, versions, 0, |versions| - 1)
+}
 
-//   predicate Valid()
-//     reads this, Repr
-//   {
-//     time >= 0 && |roots| > 0 &&
-//     (forall r :: r in roots && r != null ==> r in Repr && Repr >= r.Repr && r.Valid()) // it is a bit weird not being able to write only "Repr >= r.Repr && r.Valid()""
-//   }
-
-//   constructor Init()
-//     ensures Valid()
-//   {
-//     roots := [null];
-//     time := 0;
-//     Repr := {};
-//   }
-  
-//   // method Insert(value: int)
-//   //   requires Valid()
-//   //   modifies this, Repr
-//   //   ensures Valid()
-//   // {
-//   //   time := time + 1;
-//   //   var root := roots[|roots| - 1];
-//   //   if root == null {
-//   //     var node := new Node.Init(time, value);
-//   //     roots := roots + [node];
-//   //     Repr := Repr + {node};
-//   //     assert Repr >= node.Repr;
-//   //   } else {
-//   //     var newNode := root.Insert(time, value);
-//   //     roots := roots + [root];
-//   //     Repr := Repr + {newNode} + newNode.Repr;
-//   //     assert Repr >= newNode.Repr;
-//   //   }
-//   // }
+// lemma Test(versions1: seq<int>, versions2: seq<int>) 
+//   requires |versions2| >= |versions1| 
+//   requires Sorted(versions1) && Sorted(versions2)
+//   requires forall i | 0 <= i < |versions1| :: versions1[i] == versions2[i]
+//   // ensures forall v :: VersionIndex(v, versions1) == -1 <==> VersionIndex(v, versions2) == -1
+//   ensures |versions2| > |versions1| ==> 
+//           forall v | v < versions2[|versions1|] :: 
+//             VersionIndex(v, versions1) == VersionIndex(v, versions2)
+//   ensures |versions2| == |versions1| ==>
+//           forall v :: VersionIndex(v, versions1) == VersionIndex(v, versions2)
+// {
+//   // assert forall v | v <= versions1[|versions1| - 1] :: true;
 // }
+
+
+  predicate Sorted(s: seq<int>) 
+{
+  (forall i, j | 0 <= i < j < |s| :: 0 <= s[i] < s[j])
+  && (forall i | 0 <= i < |s| :: 0 <= s[i])
+}
+
+  predicate IsMaxMinVersion(queryVersion: int, maxMinVersion: int, versions: seq<int>)
+{
+  maxMinVersion <= queryVersion
+  && (maxMinVersion == -1 
+      || (maxMinVersion in versions
+          && forall v <- versions :: v < maxMinVersion || v == maxMinVersion || v > queryVersion))
+}
 
 class Node {
   ghost var Repr: set<Node>
@@ -53,164 +81,161 @@ class Node {
   var valuesVersions: seq<int>
   var values: seq<int>
 
-  // Consistently use A && B ==> C when I wrote A ==> B ==> C
-  ghost predicate Valid() 
+  ghost  predicate isBST(version: int)  
+    reads {this} + (set x | x in rights) + (set x | x in lefts)
+    requires |valuesVersions| > 0 && version >= valuesVersions[0]
+    requires BasicProp()
+    requires Sorted(leftsVersions) && Sorted(rightsVersions) && Sorted(ValueSetsVersions) && Sorted(valuesVersions)
+    requires forall r <- rights | r != null :: r.BasicProp() && Sorted(r.ValueSetsVersions)
+    requires forall l <- lefts | l != null :: l.BasicProp() && Sorted(l.ValueSetsVersions)
+  {
+    var v := ValueAt(version);
+    var r := RightAt(version);
+    var l := LeftAt(version);
+    // COMMENT: times out if written in a recursive fashion, i.e., r != null ==> r.isBST() && ...)
+    (r != null ==> forall v' <- r.ValueSetAt(version) :: v' > v)
+    && (l != null ==> forall v' <- l.ValueSetAt(version) :: v' < v)
+  }
+
+  ghost predicate BinarySearchProp()
+    reads {this} + (set x | x in lefts) + (set x | x in rights)
+    requires |valuesVersions| > 0
+    requires BasicProp()
+    requires Sorted(leftsVersions) && Sorted(rightsVersions) && Sorted(ValueSetsVersions) && Sorted(valuesVersions)
+    requires forall r <- rights | r != null :: r.BasicProp() && Sorted(r.ValueSetsVersions)
+    requires forall l <- lefts | l != null :: l.BasicProp() && Sorted(l.ValueSetsVersions)
+  {
+    forall v | v >= valuesVersions[0] :: isBST(v)
+  }
+
+  // ghost predicate SortedProp()
+  //   reads this
+  // {
+  //   Sorted(ValueSetsVersions) && Sorted(valuesVersions) && Sorted(leftsVersions) && Sorted(rightsVersions) 
+  // }
+
+  ghost predicate ReprProp()
     reads this, Repr
   {
-    |values| == |valuesVersions|
-    && |lefts| == |leftsVersions|
-    && |rights| == |rightsVersions|
-    && |ValueSetsVersions| == |ValueSets|
-    && |ValueSetsVersions| >= |valuesVersions| + |rightsVersions| + |leftsVersions| // Different performance if written as && |ValueSets| >= |values| + |rights| + |lefts|
-    && Sorted(ValueSetsVersions) && Sorted(valuesVersions) && Sorted(leftsVersions) && Sorted(rightsVersions) 
-    && |values| > 0 
-    && |ValueSets| > 0
     && this in Repr
     && (forall l <- lefts | l != null ::
-        l in Repr && this !in l.Repr && l.Repr < Repr && l.Valid()) 
+        l in Repr && this !in l.Repr && l.Repr < Repr && l.ReprProp() 
+        && l.BasicProp() && l.VersionsProp() && l.ValueSetProp() && l.BinarySearchProp()) 
     && (forall r <- rights | r != null ::
-        r in Repr && this !in r.Repr && r.Repr < Repr && r.Valid()) 
+        r in Repr && this !in r.Repr && r.Repr < Repr && r.ReprProp() 
+        && r.BasicProp() && r.VersionsProp() && r.ValueSetProp() && r.BinarySearchProp()) 
     // the two strong assumption does not hold for fat node method in general
-    && (forall l1 <- lefts, l2 <- lefts | l1 != null && l2 != null && l1 != l2 ::
-        l1.Repr !! l2.Repr)
-    && (forall r1 <- rights, r2 <- rights | r1 != null && r2 != null && r1 != r2 ::
-        r1.Repr !! r2.Repr)
+    // && (forall l1 <- lefts, l2 <- lefts | l1 != null && l2 != null && l1 != l2 ::
+    //     l1.Repr !! l2.Repr)
+    // && (forall r1 <- rights, r2 <- rights | r1 != null && r2 != null && r1 != r2 ::
+    //     r1.Repr !! r2.Repr)
     && (forall r <- rights, l <- lefts | r != null && l != null :: 
         l != r && l.Repr !! r.Repr) 
-    && (forall node <- Repr :: 
-          (node == this)
-          || (exists l | l in lefts && l != null :: node in l.Repr)
-          || (exists r | r in rights && r != null :: node in r.Repr))
-    && (forall rv <- rightsVersions, lv <- leftsVersions :: rv != lv)
-    // binary search tree property
-    && (forall l <- lefts | l != null ::
-          forall ls <- l.ValueSets, lv <- ls, v <- values :: lv < v)
-    && (forall r <- rights | r != null ::
-          forall rs <- r.ValueSets, rv <- rs, v <- values :: rv > v)
-    // all timestmps are larger than created
-    && (|leftsVersions| > 0 ==> leftsVersions[0] >= 0) 
-    && (|rightsVersions| > 0 ==> rightsVersions[0] >= 0) 
-    && (valuesVersions[0] >= 0) 
-    && (ValueSetsVersions[0] == valuesVersions[0])
-    // values and ValueSets
-    && (forall i | 0 <= i < |valuesVersions| ::
-          exists j | i <= j < |ValueSetsVersions| ::
-            valuesVersions[i] == ValueSetsVersions[j])
-    && (forall i | 0 <= i < |leftsVersions| ::
-          exists j | i <= j < |ValueSetsVersions| ::
-            leftsVersions[i] == ValueSetsVersions[j])
-    && (forall i | 0 <= i < |rightsVersions| ::
-          exists j | i <= j < |ValueSetsVersions| ::
-            rightsVersions[i] == ValueSetsVersions[j])
-    && (forall i | 0 <= i < |ValueSetsVersions| ::
-          ((exists j | 0 <= j <= i < |valuesVersions| :: valuesVersions[j] == ValueSetsVersions[i])
-          || (exists j | 0 <= j <= i < |leftsVersions| :: leftsVersions[j] == ValueSetsVersions[i])
-          || (exists j | 0 <= j <= i < |rightsVersions| :: rightsVersions[j] == ValueSetsVersions[i])))
   }
 
-  ghost predicate ValueSetValid()
-    reads Repr
-    requires Valid()
+  ghost predicate BasicProp()
+    reads this
   {
-    // ValueSets are union of values of its own and its left and right children
-    && (|lefts| == 0 && |rights| == 0 
-        && |ValueSetsVersions| == |ValueSets|
-        && |valuesVersions| == |values| ==>
-          |ValueSets| == |values|  
-          && forall i | 0 <= i < |ValueSetsVersions| ::
-              valuesVersions[i] == ValueSetsVersions[i] && ValueSets[i] == {values[i]})
-    && (|lefts| > 0 && |rights| == 0 
-        && |ValueSetsVersions| == |ValueSets|
-        && |leftsVersions| == |lefts|
-        && |rightsVersions| == |rights|
-        && |valuesVersions| == |values| ==>
-          forall i | 0 <= i < |ValueSetsVersions| ::
-            exists j, k | 0 <= j <= i < |leftsVersions| && 0 <= k <= i < |valuesVersions| ::
-              IsMaxMinVersion(ValueSetsVersions[i], leftsVersions[j], leftsVersions)
-              && IsMaxMinVersion(ValueSetsVersions[i], valuesVersions[k], valuesVersions)
-              // && (leftsVersions[j] == ValueSetsVersions[i] || valuesVersions[k] == ValueSetsVersions[i])
-              && (lefts[j] != null ==> 
-                    exists x | 0 <= x < |lefts[j].ValueSetsVersions| ::
-                      IsMaxMinVersion(ValueSetsVersions[i], lefts[j].ValueSetsVersions[x], lefts[j].ValueSetsVersions) 
-                      && |lefts[j].ValueSetsVersions| == |lefts[j].ValueSets| // to speed up well-formedness check
-                      && ValueSets[i] == {values[k]} + lefts[j].ValueSets[x])
-              && (lefts[j] == null ==> ValueSets[i] == {values[k]})) 
-    && (|rights| > 0 && |lefts| == 0
-        && |ValueSetsVersions| == |ValueSets|
-        && |leftsVersions| == |lefts|
-        && |rightsVersions| == |rights|
-        && |valuesVersions| == |values| ==>
-          forall i | 0 <= i < |ValueSetsVersions| ::
-            exists j, k | 0 <= j <= i < |rightsVersions| && 0 <= k <= i < |valuesVersions| ::
-              IsMaxMinVersion(ValueSetsVersions[i], rightsVersions[j], rightsVersions)
-              && IsMaxMinVersion(ValueSetsVersions[i], valuesVersions[k], valuesVersions)
-              // && (rightsVersions[k] == ValueSetsVersions[i] || valuesVersions[j] == ValueSetsVersions[i])
-              && (rights[j] != null ==> 
-                    exists x | 0 <= x < |rights[j].ValueSetsVersions| ::
-                          IsMaxMinVersion(ValueSetsVersions[i], rights[j].ValueSetsVersions[x], rights[j].ValueSetsVersions) 
-                          && |rights[j].ValueSetsVersions| == |rights[j].ValueSets| // to speed up well-formedness check
-                          && ValueSets[i] == {values[k]} + rights[j].ValueSets[x])
-              && (rights[j] == null ==> ValueSets[i] == {values[k]})) 
-    && (|rights| > 0 && |lefts| > 0
-        && |ValueSetsVersions| == |ValueSets|
-        && |leftsVersions| == |lefts|
-        && |rightsVersions| == |rights|
-        && |valuesVersions| == |values| ==>
-          forall i | 0 <= i < |ValueSetsVersions| ::
-            exists j, k, l | 0 <= j <= i < |values| && 0 <= k <= i < |rights| && 0 <= l <= i < |lefts| ::
-              IsMaxMinVersion(ValueSetsVersions[i], valuesVersions[i], valuesVersions)
-              && IsMaxMinVersion(ValueSetsVersions[i], rightsVersions[k], rightsVersions)
-              && IsMaxMinVersion(ValueSetsVersions[i], leftsVersions[l], leftsVersions)
-              // && (rightsVersions[k] == ValueSetsVersions[i]
-              //   || leftsVersions[l] == ValueSetsVersions[i] 
-              //   || valuesVersions[j] == ValueSetsVersions[i])
-              && (lefts[l] != null && rights[k] != null ==> 
-                    exists x, y | 0 <= x < |lefts[l].ValueSetsVersions| && 0 <= y < |rights[k].ValueSetsVersions| ::
-                      IsMaxMinVersion(ValueSetsVersions[i], lefts[l].ValueSetsVersions[x], lefts[l].ValueSetsVersions)
-                      && IsMaxMinVersion(ValueSetsVersions[i], rights[k].ValueSetsVersions[y], rights[k].ValueSetsVersions)
-                      && |lefts[l].ValueSetsVersions| == |lefts[l].ValueSets| // to speed up well-formedness check
-                      && |rights[k].ValueSetsVersions| == |rights[k].ValueSets| // to speed up well-formedness check 
-                      &&  ValueSets[i] == {values[j]} + lefts[l].ValueSets[x] + rights[k].ValueSets[y])
-              && (lefts[l] != null && rights[k] == null ==> 
-                    exists x | 0 <= x < |lefts[l].ValueSetsVersions| ::
-                      IsMaxMinVersion(ValueSetsVersions[i], lefts[l].ValueSetsVersions[x], lefts[l].ValueSetsVersions)
-                      && |lefts[l].ValueSetsVersions| == |lefts[l].ValueSets| // to speed up well-formedness check
-                      && ValueSets[i] == {values[j]} + lefts[l].ValueSets[x])
-              && (rights[k] != null && lefts[l] == null ==> 
-                    exists x | 0 <= x < |rights[k].ValueSetsVersions| ::
-                      IsMaxMinVersion(ValueSetsVersions[i], rights[k].ValueSetsVersions[x], rights[k].ValueSetsVersions)
-                      && |rights[k].ValueSetsVersions| == |rights[k].ValueSets| // to speed up well-formedness check 
-                      &&  ValueSets[i] == {values[j]} + rights[k].ValueSets[x])
-              && (rights[k] == null && lefts[l] == null ==> ValueSets[i] == {values[j]})) 
+    |ValueSetsVersions| == |ValueSets|
+    && |valuesVersions| == |values|
+    && |leftsVersions| == |lefts|
+    && |rightsVersions| == |rights|
+    && |ValueSetsVersions| > 0
+    && |valuesVersions| > 0
+    && |ValueSetsVersions| <= |leftsVersions| + |rightsVersions| + |valuesVersions|
+    && ValueSetsVersions[0] == valuesVersions[0]
+    && ValueSetsVersions[0] >= 0 
+    && (|leftsVersions| > 0 ==> leftsVersions[0] > 0)
+    && (|rightsVersions| > 0 ==> rightsVersions[0] > 0)
+    && Sorted(ValueSetsVersions) && Sorted(valuesVersions) && Sorted(leftsVersions) && Sorted(rightsVersions) 
   }
 
-  predicate Sorted(s: seq<int>) 
+  ghost predicate ValueSetUnions(v: int)
+    reads {this} + (set x | x in rights) + (set x | x in lefts)
+    requires |valuesVersions| > 0 && v >= valuesVersions[0]
+    requires BasicProp()
+    requires Sorted(leftsVersions) && Sorted(rightsVersions) && Sorted(ValueSetsVersions) && Sorted(valuesVersions)
+    requires forall r <- rights | r != null :: r.BasicProp() && Sorted(r.ValueSetsVersions)
+    requires forall l <- lefts | l != null :: l.BasicProp() && Sorted(l.ValueSetsVersions)
   {
-    (forall i, j | 0 <= i < j < |s| :: 0 <= s[i] < s[j])
-    && (forall i | 0 <= i < |s| :: 0 <= s[i])
+     ValueSetAt(v) == {ValueAt(v)} + LeftValueSetAt(v) + RightValueSetAt(v)
   }
 
-  predicate IsMaxMinVersion(version: int, maxMinVersion: int, versions: seq<int>)
-    // requires Sorted(versions)
+  ghost predicate ValueSetProp()
+    reads {this} + (set x | x in lefts) + (set x | x in rights)
+    requires VersionsProp() && BasicProp() 
+    requires forall l <- lefts | l != null :: l.BasicProp() && Sorted(l.ValueSetsVersions)
+    requires forall r <- rights | r != null :: r.BasicProp() && Sorted(r.ValueSetsVersions)
   {
-    maxMinVersion <= version
-    && (maxMinVersion == -1 
-        || (maxMinVersion in versions
-            && forall v <- versions :: v < maxMinVersion || v == maxMinVersion || v > version))
+    // COMMENT: using forall v | ValueSetsVersions[0] <= v <= ValueSetsVersions[|ValueSetsVersions| - 1] did not work
+    (forall v | valuesVersions[0] <= v :: ValueSetUnions(v))
   }
+
+  ghost predicate VersionsProp()
+    reads {this} + (set x | x in lefts) + (set x | x in rights)
+  {
+    (forall v <- ValueSetsVersions ::
+        v in valuesVersions 
+        || (exists l <- lefts :: l != null && v in l.ValueSetsVersions)
+        || (exists r <- rights :: r != null && v in r.ValueSetsVersions))
+    && (valuesVersions <= ValueSetsVersions)
+    && (leftsVersions <= ValueSetsVersions)
+    && (forall l <- lefts | l != null :: 
+          l.ValueSetsVersions < ValueSetsVersions)
+    && (rightsVersions <= ValueSetsVersions)
+    && (forall r <- rights | r != null :: 
+          r.ValueSetsVersions < ValueSetsVersions)
+  }
+
+  ghost function LeftValueSetAt(version: int) : (res: set<int>)
+    reads {this} + (set x | x in lefts)
+    requires BasicProp() && Sorted(leftsVersions)
+    requires forall l <- lefts | l != null :: l.BasicProp() && Sorted(l.ValueSetsVersions)
+    ensures LeftAt(version) == null ==> res == {}
+    ensures LeftAt(version) != null ==> res == LeftAt(version).ValueSetAt(version)
+  {
+    var l := LeftAt(version);
+    if l == null then
+      {}
+    else
+      l.ValueSetAt(version)
+  }
+
+  ghost function RightValueSetAt(version: int) : (res: set<int>)
+    reads {this} + (set x | x in rights)
+    requires BasicProp() && Sorted(rightsVersions)
+    requires forall r <- rights | r != null :: r.BasicProp() && Sorted(r.ValueSetsVersions)
+    ensures RightAt(version) == null ==> res == {}
+    ensures RightAt(version) != null ==> res == RightAt(version).ValueSetAt(version)
+  {
+    var r := RightAt(version);
+    if r == null then
+      {}
+    else
+      r.ValueSetAt(version)
+  }
+
+  lemma VersionsLemma(version: int)
+    requires ReprProp() && VersionsProp() && BasicProp()
+    requires version > ValueSetsVersions[|ValueSetsVersions| - 1]
+    ensures |rightsVersions| == 0 || version > rightsVersions[|rightsVersions| - 1]
+    ensures forall r <- rights | r != null :: version > r.ValueSetsVersions[|r.ValueSetsVersions| - 1]
+    ensures forall l <- lefts | l != null :: version > l.ValueSetsVersions[|l.ValueSetsVersions| - 1]
+  {}
 
   constructor Init(time: int, value: int)
-    requires time > 0
-    ensures Valid() && fresh(Repr)
+    requires time >= 0
+    ensures fresh(Repr)
     ensures lefts == []
-    ensures leftsVersions == []
     ensures rights == []
-    ensures rightsVersions == []
     ensures Repr == {this}
     ensures values == [value]
     ensures valuesVersions == [time]
     ensures ValueSets == [{value}]
     ensures ValueSetsVersions == [time]
+    ensures ValueSetAt(time) == {value}
+    // ensures forall v | v >= time :: ValueAt(v) == value
+    ensures ReprProp() && VersionsProp() && BasicProp() && ValueSetProp() && BinarySearchProp() 
   {
     lefts := [];
     leftsVersions := [];
@@ -223,10 +248,10 @@ class Node {
     ValueSets := [{value}];
   }
 
-  function {:opaque} Left(): (l: Node?)
-    reads Repr 
-    requires Valid()
-    ensures l != null ==> l in lefts && l.Valid()
+  function Left(): (l: Node?)
+    reads this
+    ensures |lefts| == 0 ==> l == null
+    ensures |lefts| > 0 ==> l == lefts[|lefts| - 1]
   {
     if |lefts| > 0 then
       lefts[|lefts| - 1]
@@ -234,10 +259,10 @@ class Node {
       null
   }
 
-  function {:opaque} Right(): (r: Node?)
-    reads Repr 
-    requires Valid()
-    ensures r != null ==>r in rights && r.Valid() 
+  function Right(): (r: Node?)
+    reads this
+    ensures |rights| == 0 ==> r == null
+    ensures |rights| > 0 ==> r == rights[|rights| - 1]
   {
     if |rights| > 0 then
       rights[|rights| - 1]
@@ -245,334 +270,410 @@ class Node {
       null
   }
 
-  function {:opaque} Value(): (v: int)
+  function Value(): (v: int)
     reads this
     requires |values| > 0
-    ensures v in values
+    ensures v == values[|values| - 1]
   {
     values[|values| - 1]
   }
 
-  ghost function{:opaque}  ValueSet(): (s: set<int>)
-    reads Repr
-    requires Valid()
-    ensures s in ValueSets
+  ghost function ValueSet(): (s: set<int>)
+    reads this
+    requires |ValueSets| > 0
+    ensures s == ValueSets[|ValueSets| - 1]
   {
     ValueSets[|ValueSets| - 1]
   }
 
-  function {:opaque} MaxMinVersionIndexHelper(version: int, versions: seq<int>, lo: int, hi: int): (index: int)
-    decreases hi - lo
-    requires |versions| == 0 ==> lo > hi && hi == -1
-    requires 0 <= lo <= |versions| 
-    requires -1 <= hi < |versions|
-    requires lo <= hi + 1
-    requires Sorted(versions)
-    requires forall k :: hi < k < |versions| ==> versions[k] > version
-    requires forall k :: 0 <= k < lo ==> versions[k] <= version
-    ensures -1 <= index < |versions|
-    ensures index == -1 <==> (|versions| == 0 || forall k :: 0 <= k < |versions| ==> versions[k] > version)
-    ensures index >= 0 <==> |versions| > 0 && versions[0] <= version
-    ensures index == -1 || versions[index] <= version
-    ensures forall i | 0 <= i < index :: versions[i] < version
-    ensures index >= 0 ==> forall i | index < i < |versions| :: versions[i] > version
-  {
-    if (lo > hi) then
-      assert lo <= 0 || versions[lo - 1] <= version;
-      lo - 1
-    else
-      assert |versions| > 0;
-      var mid := lo + (hi - lo) / 2;
-      var v := versions[mid];
-      if v == version then
-        mid
-      else if v < version then
-        MaxMinVersionIndexHelper(version, versions, mid + 1, hi)
-      else 
-        MaxMinVersionIndexHelper(version, versions, lo, mid - 1)
-  } 
-
-  function {:opaque} MaxMinVersionIndex(version: int, versions: seq<int>): (index: int)
-    requires Sorted(versions)
-    ensures -1 <= index < |versions|
-    ensures index >= 0 <==> |versions| > 0 && versions[0] <= version
-    ensures index == -1 || IsMaxMinVersion(version, versions[index], versions)
-  {
-    MaxMinVersionIndexHelper(version, versions, 0, |versions| - 1)
-  }
-
-  ghost function {:opaque} MaxMinVersionIndexForValueSets(version: int) : (index: int)
+  ghost function {:opaque} VersionIndexForValueSets(version: int) : (index: int)
     reads this
     requires Sorted(ValueSetsVersions)
-    requires |ValueSetsVersions| > 0
     ensures -1 <= index < |ValueSetsVersions|
-    ensures index >= 0 <==> ValueSetsVersions[0] <= version
+    ensures index >= 0 <==> |ValueSetsVersions| > 0 && ValueSetsVersions[0] <= version
     ensures index == -1 || IsMaxMinVersion(version, ValueSetsVersions[index], ValueSetsVersions)
+    ensures version in ValueSetsVersions <==> index >= 0 && |ValueSetsVersions| > index && ValueSetsVersions[index] == version
+    ensures index == VersionIndex(version, ValueSetsVersions)
   {
-    MaxMinVersionIndex(version, ValueSetsVersions)
+    VersionIndex(version, ValueSetsVersions)
   }
 
-  ghost function {:opaque} ValueSetAtVersion(version: int) : (res: set<int>)
-    reads Repr
-    requires Valid()
-    ensures Valid()
-    ensures MaxMinVersionIndexForValueSets(version) >= 0 ==> 
-              res == ValueSets[MaxMinVersionIndexForValueSets(version)]
+  ghost function {:opaque} ValueSetAt(version: int) : (res: set<int>)
+    reads this
+    requires Sorted(ValueSetsVersions)
+    requires |ValueSetsVersions| == |ValueSets|
+    ensures VersionIndexForValueSets(version) == -1 ==> res == {}
+    ensures VersionIndexForValueSets(version) >= 0 ==> res in ValueSets
+    ensures VersionIndexForValueSets(version) == -1 
+            || res == ValueSets[VersionIndexForValueSets(version)]
+
   {
-    var i := MaxMinVersionIndexForValueSets(version);
+    var i := VersionIndexForValueSets(version);
     if i == -1 then
       {}
     else
       ValueSets[i]
   }
 
-  function {:opaque} MaxMinVersionIndexForValues(version: int) : (index: int)
-    reads Repr
-    requires Valid()
+  function {:opaque} VersionIndexForValues(version: int) : (index: int)
+    reads this
+    requires Sorted(valuesVersions)
     ensures -1 <= index < |valuesVersions|
-    ensures index >= 0 ==> IsMaxMinVersion(version, valuesVersions[index], valuesVersions)
-    ensures index >= 0 ==> valuesVersions[index] in ValueSetsVersions
-    ensures index <= MaxMinVersionIndexForValueSets(version)
+    // ensures index == -1 <=> |valuesVersions| == 0 && valuesVersions[0] > version
+    ensures index >= 0 <==> |valuesVersions| > 0 && valuesVersions[0] <= version
+    ensures index == -1 || IsMaxMinVersion(version, valuesVersions[index], valuesVersions)
+    ensures index == VersionIndex(version, valuesVersions)
+    // ensures index == -1 || valuesVersions[index] in ValueSetsVersions
+    // ensures index <= VersionIndexForValueSets(version)
   {
-    var index := MaxMinVersionIndex(version, valuesVersions);
-    if index >= 0 then
-      assert exists i | 0 <= i < |ValueSetsVersions| :: 
-              ValueSetsVersions[i] == valuesVersions[index] 
-              && i >= index;
-      index
-    else
-      index
+    VersionIndex(version, valuesVersions)
   }
 
-  function {:opaque} ValueAtVersion(version: int): (res: int)
-    reads Repr 
-    requires Valid() && ValueSetValid()
-    ensures Valid()
-    ensures MaxMinVersionIndexForValues(version) >= 0 ==> 
-          res == values[MaxMinVersionIndexForValues(version)]
+  function {:opaque} ValueAt(version: int): (res: int)
+    reads this
+    requires Sorted(valuesVersions) && |valuesVersions| == |values|
+    ensures VersionIndexForValues(version) >= 0 ==> res in values
+    ensures VersionIndexForValues(version) == -1
+            || res == values[VersionIndexForValues(version)]
+    // ensures VersionIndexForValues(version) == -1 ||
+    //         res in ValueSetAt(version)
   {
-    var i := MaxMinVersionIndexForValues(version);
+    var i := VersionIndexForValues(version);
     if i == -1 then
       -1
     else
-      if |lefts| == 0 then
-        if |rights| == 0 then
-          assert values[i] in ValueSetAtVersion(version);
-          values[i]
-        else
-          assert values[i] in ValueSetAtVersion(version);
-          values[i]
-      else
-        assert values[i] in ValueSetAtVersion(version);
-        values[i]
+      values[i]
   }
 
-  function MaxMinVersionIndexForRights(version: int) : (res: int)
-    reads Repr
-    requires Valid()
-    ensures -1 <= res < |rights|
-    ensures res == -1 && |rights| > 0 ==> rightsVersions[0] > version
-    ensures res >= 0 ==> MaxMin(version, res, rightsVersions)
-    ensures res >= 0 ==> rightsVersions[res] in ValueSetsVersions
-    ensures res <= MaxMinVersionIndexForValueSets(version)
+  function {:opaque} VersionIndexForRights(version: int) : (index: int)
+    reads this
+    requires Sorted(rightsVersions)
+    ensures -1 <= index < |rightsVersions|
+    ensures index >= 0 <==> |rightsVersions| > 0 && rightsVersions[0] <= version
+    ensures index == -1 || IsMaxMinVersion(version, rightsVersions[index], rightsVersions)
+    ensures index == VersionIndex(version, rightsVersions)
+    // ensures index == -1 || rightsVersions[index] in ValueSetsVersions
+    // ensures index <= VersionIndexForValueSets(version)
   {
-    MaxMinVersion(version, rightsVersions)
+    VersionIndex(version, rightsVersions)
   }
 
-  // function RightAtVersion(version: int): (res: Node?)
-  //   requires Valid()
-  //   reads Repr 
-  //   ensures res != null ==> res.Valid()
-  //   ensures res != null ==> res.ValueSetAtVersion(version) <= ValueSetAtVersion(version)
-  // {
-  //   var i := MaxMinVersionIndexForRights(version);
-  //   if i == -1 then
-  //     null
-  //   else
-  //     rights[i]
-  // }
+  function {:opaque} RightAt(version: int) : (res: Node?)
+    reads this
+    requires Sorted(rightsVersions) && |rightsVersions| == |rights|
+    ensures res == null || res in rights
+    ensures VersionIndexForRights(version) >= 0 ==> res in rights
+    ensures VersionIndexForRights(version) == -1 ==> res == null
+    ensures VersionIndexForRights(version) == -1 
+            || res == rights[VersionIndexForRights(version)]
+  {
+    var i := VersionIndexForRights(version);
+    if i == -1 then
+      null
+    else
+      rights[i]
+  }
 
-  // function {:opaque} MaxMinVersionIndexForLefts(version: int) : (res: int)
-  //   reads Repr
-  //   requires Valid()
-  //   ensures -1 <= res < |leftsVersions|
-  //   ensures res == -1 && |leftsVersions| > 0 ==> leftsVersions[0] > version
-  //   ensures res >= 0 ==> MaxMin(version, res, leftsVersions)
-  //   ensures res >= 0 ==> leftsVersions[res] in ValueSetsVersions
-  //   ensures res <= MaxMinVersionIndexForValueSets(version)
-  // {
-  //   MaxMinVersionIndex(version, leftsVersions)
-  // }
-  
-  // function {:opaque} LeftAtVersion(version: int): (res: Node?)
-  //   reads Repr
-  //   requires Valid()
-  //   ensures res != null ==> res in lefts && res.Valid()
-  //   ensures res != null ==> res.ValueSetAtVersion(version) <= ValueSetAtVersion(version)
-  // {
-  //   var i := MaxMinVersionIndexForLefts(version);
-  //   if i == -1 then
-  //     null
-  //   else
-  //     lefts[i]
-  // }
+  function {:opaque} VersionIndexForLefts(version: int) : (index: int)
+    reads this
+    requires Sorted(leftsVersions)
+    ensures -1 <= index < |leftsVersions|
+    ensures index >= 0 <==> |leftsVersions| > 0 && leftsVersions[0] <= version
+    ensures index == -1 || IsMaxMinVersion(version, leftsVersions[index], leftsVersions)
+    ensures index == VersionIndex(version, leftsVersions)
+    // ensures index == -1 || leftsVersions[index] in ValueSetsVersions
+    // ensures index <= VersionIndexForValueSets(version)
+  {
+    VersionIndex(version, leftsVersions)
+  }
 
-  // function Find(version: int, value: int): (found: bool)
-  //   requires Valid()
-  //   reads Repr
-  //   decreases Repr
-  //   // ensures found ==> value in ValueSetAtVersion(version).1
-  //   // ensures value in ValueSetAtVersion(version).1 ==> found
-  // {
+  function {:opaque} LeftAt(version: int) : (res: Node?)
+    reads this
+    requires Sorted(leftsVersions) && |leftsVersions| == |lefts|
+    ensures res == null || res in lefts
+    ensures VersionIndexForLefts(version) >= 0 ==> res in lefts
+    ensures VersionIndexForLefts(version) == -1 ==> res == null
+    ensures VersionIndexForLefts(version) == -1 
+            || res == lefts[VersionIndexForLefts(version)]
+  {
+    var i := VersionIndexForLefts(version);
+    if i == -1 then
+      null
+    else
+      lefts[i]
+  }
 
-  //   if MaxMinVersionIndexForValues(version) == -1 then 
-  //     false
-  //   else
-  //     var x := ValueAtVersion(version);
-  //     if x > value then
-  //       var left := LeftAtVersion(version);
-  //       if left == null then
-  //         false
-  //       else
-  //         assert |lefts| > 0;
-  //         var lf := left.Find(version, value);
-  //         lf
-  //     else if x < value then
-  //       var right := RightAtVersion(version);
-  //       if right == null then
-  //         false
-  //       else
-  //         assert |rights| > 0;
-  //         var rf := right.Find(version, value);
-  //         rf
-  //     else
-  //       // assert value in ValueSetAtVersion(version);
-  //       true
-  // }
+  function {:opaque} Find(version: int, value: int) : (res: bool) 
+    reads Repr
+    requires version >= 0
+    requires ReprProp() && VersionsProp() && BasicProp() && ValueSetProp() && BinarySearchProp()
+    ensures res <==> value in ValueSetAt(version)
+  {
+    var i := VersionIndexForValues(version);
+    if i == -1 then
+      assert VersionIndexForValueSets(version) == -1;
+      assert value !in ValueSetAt(version);
+      false
+    else
+      assert version >= valuesVersions[0];
+      assert isBST(version);  // COMMENT: crutial
+      assert ValueSetUnions(version); // COMMENT: crutial
+      var x := ValueAt(version);
+      if x > value then
+        var left := LeftAt(version);
+        ghost var r := RightAt(version);
+        assert r != null ==> value !in r.ValueSetAt(version);
+        if left == null then 
+          false
+        else
+          left.Find(version, value)
+      else if x < value then
+        var right := RightAt(version);
+        ghost var l := LeftAt(version);
+        assert l != null ==> value !in l.ValueSetAt(version);
+        if right == null then
+          false
+        else
+          right.Find(version, value)
+      else
+        true
+  }
 
-  // method Insert(time: int, value: int) returns (node: Node?)
-  //   requires Valid()
-  //   requires time > 0
-  //   requires removed == -1
-  //   requires time > ValueSets[|ValueSets| - 1].0
-  //   modifies Repr
-  //   decreases Repr
-  //   ensures node == null ==> 
-  //     Repr == old(Repr)
-  //   ensures node != null ==> 
-  //     fresh(node) &&
-  //     node.Repr == {node} && 
-  //     Repr == old(Repr) + {node} &&
-  //     node.Valid()
-  //   // ensures ValueSetAtVersion(time).0 != -1
-  //   // ensures value in ValueSetAtVersion(time).1
-  //   // ensures Valid()
+  // method AddNode(node: Node?, addToRight: bool)
+  //   modifies this
+  //   requires node != null ==> node !in Repr
+  //   requires node != null ==> 
+  //     node.lefts == []
+  //     && node.rights == []
+  //     && node.Repr == {node}
+  //     && |node.values| == 1 
+  //     && |node.ValueSets| == 1
+  //     && node.ReprProp() 
+  //     && node.VersionsProp() 
+  //     && node.BasicProp() 
+  //     && node.ValueSetProp() 
+  //     && node.BinarySearchProp()
+  //   requires node != null && addToRight ==> AllSmallerThan(values, node.ValueSets)
+  //   requires node != null && !addToRight ==> AllBiggerThan(values, node.ValueSets)
+  //   requires ReprProp() && VersionsProp() && BasicProp() && ValueSetProp() && BinarySearchProp() 
+  //   requires node != null ==> node.valuesVersions[0] > ValueSetsVersions[|ValueSetsVersions| - 1]
+  //   ensures node != null ==> Repr == old(Repr) + {node}
+  //   ensures node != null && addToRight ==> rights == old(rights) + [node] && lefts == old(lefts)
+  //   ensures node != null && !addToRight ==> lefts == old(lefts) + [node] && rights == old(rights)
+  //   ensures node == null <==> Repr == old(Repr)
+  //   ensures ReprProp() && VersionsProp() && BasicProp() && ValueSetProp() && BinarySearchProp() 
+  //   ensures node != null ==> node.values[0] in ValueSetAt(node.valuesVersions[0]) 
   // {
-  //   var x := Value();
-  //   if x < value {
-  //     var r := Right();
-  //     if r == null {
-  //       node := new Node.Init(time, value);
-  //       assert node.Valid();
-  //       rights := rights + [(time, node)];
-  //       Repr := Repr + node.Repr;
-  //       ValueSets := ValueSets + [(time, {x} + ValueSets[|ValueSets| - 1].1)];
+  //   if (node != null) {
+  //     var version := node.valuesVersions[0];
+  //     ghost var value := node.values[0];
+  //     if (addToRight) {
+  //       assert |rightsVersions| > 0 ==> rightsVersions[|rightsVersions| - 1] in ValueSetsVersions;
+  //       assert |rightsVersions| > 0 ==> version > rightsVersions[|rightsVersions| - 1];
+  //       rights := rights + [node];
+  //       rightsVersions := rightsVersions + [version];
+  //       assert leftsVersions == old(leftsVersions);
+  //       assert rightsVersions == old(rightsVersions) + [version];
   //     } else {
-  //       node := r.Insert(time, value);
-  //       if (node != null) {
-  //         assert node.Valid();
-  //         Repr := Repr + node.Repr;
-  //         ValueSets := ValueSets + [(time, {x} + ValueSets[|ValueSets| - 1].1)];
-  //       } 
+  //       assert |leftsVersions| > 0 ==> leftsVersions[|leftsVersions| - 1] in ValueSetsVersions;
+  //       assert |leftsVersions| > 0 ==> version > leftsVersions[|leftsVersions| - 1];
+  //       lefts := lefts + [node];
+  //       leftsVersions := leftsVersions + [version];
+  //       assert rightsVersions == old(rightsVersions);
+  //       assert leftsVersions == old(leftsVersions) + [version];
   //     }
-  //   } else if x > value {
-  //     var l := Left();
-  //     if l == null {
-  //       node := new Node.Init(time, value);
-  //       assert node.Valid();
-  //       lefts := lefts + [(time, node)];
-  //       Repr := Repr + node.Repr;
-  //       ValueSets := ValueSets + [(time, {x} + ValueSets[|ValueSets| - 1].1)];
-  //     } else {
-  //       node := l.Insert(time, value);
-  //       if (node != null) {
-  //         assert node.Valid();
-  //         // assert (forall r <- rights | r.1 != null :: r.1 !in l.Repr);  
-  //         // assert (forall r <- rights | r.1 != null :: r.1 in Repr && r.1.Repr < Repr && this !in r.1.Repr && r.1.Valid());
-  //         Repr := Repr + node.Repr;
-  //         ValueSets := ValueSets + [(time, {x} + ValueSets[|ValueSets| - 1].1)];
-  //       } 
-  //     }
-  //   } else {
-  //     node := null;
-  //   }
-  // }
 
-  // method DeleteMin(parent: Node, fromLeft: bool, time: int) returns (minV: int)
-  //   requires Valid() && parent.Valid()
-  //   requires parent.Left() == this || parent.Right() == this
-  //   decreases Repr
-  //   modifies parent.Repr
-  //   ensures lefts == old(lefts)
-  //   // ensures rights == old(rights)
-  //   ensures parent.Valid()
-  // {
-  //   var l := Left();
-  //   if l == null {
-  //     assert Valid();
-  //     if fromLeft {
-  //       parent.lefts := parent.lefts + [(time, Right())];
-  //     } else {
-  //       parent.rights := parent.rights + [(time, Right())];
-  //     }
-  //     assert Valid();
-  //     assert parent.Valid();
-  //     minV := Value();
-  //     assert parent.Valid();
-  //     assert lefts == old(lefts);
-  //   } else {
-  //     assert Valid();
-  //     minV := l.DeleteMin(this, true, time);
-  //     assert lefts == old(lefts);
-  //     assert Valid();
-  //     // assert parent.Valid();
-  //   }
-  // }
+  //     assert(Sorted(leftsVersions));
+  //     assert(Sorted(rightsVersions));
 
-  // method Delete(parent: Node?, fromLeft: bool, time: int, value: int) returns (root: Node?) 
-  //   requires Valid()
-  //   modifies Repr
-  //   decreases Repr
-  //   ensures root != null ==> root.Valid()
-  // {
-  //   var x := Value();
-  //   var r := Right();
-  //   var l := Left();
-  //   if x == value {
-  //     if r != null {
-  //       var minV := r.DeleteMin(this, false, time);
-  //       values := values + [(time, minV)];
-  //     } else {
-  //       if parent != null {
-  //         if fromLeft {
-  //           lefts := lefts + [(time, l)];
-  //         } else {
-  //           rights := rights + [(time, l)];
+  //     Repr := Repr + {node};
+  //     ValueSets := ValueSets + [ValueSet() + {value}];
+  //     ValueSetsVersions := ValueSetsVersions + [version];
+
+  //     assert ValueSetsVersions == old(ValueSetsVersions) + [version];
+  //     assert Sorted(ValueSetsVersions);
+
+  //     assert forall v | ValueSetsVersions[0] <= v :: ValueSetAt(v) == {ValueAt(v)} + LeftValueSetAt(v) + RightValueSetAt(v) by {
+  //         assert forall v | ValueSetsVersions[0] <= v < version :: ValueSetAt(v) == {ValueAt(v)} + LeftValueSetAt(v) + RightValueSetAt(v) by {
+  //         assert forall v | ValueSetsVersions[0] <= v < version :: ValueSetAt(v) == old(ValueSetAt(v)) by {
+  //           assert forall v | ValueSetsVersions[0] <= v < version ::
+  //                 old(VersionIndexForValueSets(v)) == VersionIndex(v, old(ValueSetsVersions))
+  //                 && VersionIndexForValueSets(v) == VersionIndex(v, ValueSetsVersions);
+  //           Test(old(ValueSetsVersions), ValueSetsVersions);
+  //           assert forall v | ValueSetsVersions[0] <= v < version :: VersionIndexForValueSets(v) == old(VersionIndexForValueSets(v));
   //         }
-  //       } else {
-  //         root := l;
-  //       }
-  //     }
-  //   } else if x < value {
-  //     if r != null {
-  //       root := r.Delete(this, false, time, value);
-  //     }
-  //   } else {
-  //     if l != null {
-  //       root := l.Delete(this, true, time, value);
-  //     }
-  //   }
 
-  //   root := this;
+  //         assert forall v | ValueSetsVersions[0] <= v < version :: LeftValueSetAt(v) == old(LeftValueSetAt(v)) by {
+  //           assert forall v | ValueSetsVersions[0] <= v < version ::
+  //                 old(VersionIndexForLefts(v)) == VersionIndex(v, old(leftsVersions))
+  //                 && VersionIndexForLefts(v) == VersionIndex(v, leftsVersions);
+  //           Test(old(leftsVersions), leftsVersions);
+  //           assert forall v | ValueSetsVersions[0] <= v < version :: VersionIndexForLefts(v) == old(VersionIndexForLefts(v));
+  //           assert forall v | ValueSetsVersions[0] <= v < version :: LeftAt(v) == old(LeftAt(v));
+  //         }
+
+  //         assert  forall v | ValueSetsVersions[0] <= v < version :: RightValueSetAt(v) == old(RightValueSetAt(v)) by {
+  //           assert forall v | ValueSetsVersions[0] <= v < version ::
+  //                 old(VersionIndexForRights(v)) == VersionIndex(v, old(rightsVersions))
+  //                 && VersionIndexForRights(v) == VersionIndex(v, rightsVersions);
+  //           Test(old(rightsVersions), rightsVersions);
+  //           assert forall v | ValueSetsVersions[0] <= v < version :: VersionIndexForRights(v) == old(VersionIndexForRights(v));
+  //           assert forall v | ValueSetsVersions[0] <= v < version :: RightAt(v) == old(RightAt(v));
+  //         }
+  //       }
+
+  //       assert forall v | version < v :: ValueSetAt(v) == ValueSetAt(version);
+  //       assert forall v | version < v :: LeftValueSetAt(v) == LeftValueSetAt(version);
+  //       assert forall v | version < v :: RightValueSetAt(v) == RightValueSetAt(version);
+
+  //       assume false;
+        
+  //       assert ValueSetAt(version) == {ValueAt(version)} + LeftValueSetAt(version) + RightValueSetAt(version) by {
+  //         assert ValueAt(version) == old(ValueAt(version));
+  //         assert !addToRight ==> (LeftAt(version) == node
+  //                               && LeftValueSetAt(version) == {value} + old(LeftValueSetAt(version)) && RightValueSetAt(version) == old(RightValueSetAt(version)));
+  //         assert addToRight ==> (RightAt(version) == node
+  //                               && RightValueSetAt(version) == {value} + old(RightValueSetAt(version)) && LeftValueSetAt(version) == old(LeftValueSetAt(version)));
+  //         assert VersionIndexForValueSets(version) == |ValueSetsVersions| - 1;
+  //         assert ValueSetAt(version) == ValueSets[|ValueSetsVersions| - 1];
+
+  //         // assert oldVS == ValueSets[|ValueSets| - 2];
+  //         // assert oldVS == old(ValueSetAt(version));
+  //         assert ValueSetAt(version) == old(ValueSetAt(version)) + {value};
+  //       }
+
+        
+
+  //     }
+
+
+  //   }
   // }
+
+  method Insert(version: int, value: int) returns (res: Node?) 
+    modifies Repr
+    decreases Repr
+    requires ReprProp() && BasicProp() && VersionsProp() && ValueSetProp() && BinarySearchProp()
+    requires version > ValueSetsVersions[|ValueSetsVersions| - 1]
+    ensures res != null ==> fresh(res) && Repr == old(Repr) + {res}
+    ensures res == null ==> Repr == old(Repr)
+    ensures BasicProp() && ReprProp()
+    // ensures res != null ==> res.ReprProp() && res.BasicProp() && res.VersionsProp() && res.ValueSetProp() && res.BinarySearchProp()
+    // ensures res != null ==> 
+    //   ValueSetsVersions == old(ValueSetsVersions) + [version]
+    //   && ValueSets == old(ValueSets) + [old(ValueSetAt(version)) + { value }]
+    // ensures value < Value() && res != null ==>
+    //   leftsVersions == old(leftsVersions) + [version]
+    //   && lefts == old(lefts) + [res]
+    //   && rightsVersions == old(rightsVersions)
+    //   && rights == old(rights)
+    // ensures value > Value() && res != null ==> 
+    //   rightsVersions == old(rightsVersions) + [version]
+    //   && rights == old(rights) + [res]
+    //   && leftsVersions == old(leftsVersions)
+    //   && lefts == old(lefts)
+    // ensures ValueSetUnions(version) 
+    // ensures forall v | ValueSetsVersions[0] <= v < version :: ValueSetAt(v) == old(ValueSetAt(v))
+    // ensures forall v | ValueSetsVersions[0] <= v < version :: LeftValueSetAt(v) == old(LeftValueSetAt(v))
+    // ensures forall v | ValueSetsVersions[0] <= v < version :: RightValueSetAt(v) == old(RightValueSetAt(v))
+    // ensures forall v | ValueSetsVersions[0] <= v < version :: ValueSetUnions(v)
+    // ensures res == null <==> Repr == old(Repr) && ValueSets == old(ValueSets) && value in old(ValueSetAt(version))
+    
+    // ensures VersionsProp() && BinarySearchProp() && ValueSetProp()
+    // ensures value in ValueSetAt(version) 
+  {
+    var x := Value();
+    if x > value {
+      assume false;
+      var left := Left();
+      if left == null { 
+        res := new Node.Init(version, value);
+      } else {
+        res := left.Insert(version, value);
+      }
+    } else if x < value {
+
+      var right := Right();
+      if right == null {
+        res := new Node.Init(version, value);
+        
+        assert Sorted(rightsVersions);
+        if (|rightsVersions| > 0) {
+          assert version > ValueSetsVersions[|ValueSetsVersions| - 1] >= rightsVersions[|rightsVersions| - 1];
+        }
+        
+        rights := rights + [res];
+        rightsVersions := rightsVersions + [version];
+
+        assert Sorted(rightsVersions);
+
+        ghost var OldValueSet := ValueSet();
+        Repr := Repr + {res};
+        ValueSets := ValueSets + [OldValueSet + {value}];
+        ValueSetsVersions := ValueSetsVersions + [version];
+
+        // assert res.ValueSets == [{value}];
+        // assert OldValueSet == old(ValueSetAt(version));
+      
+        // assert Sorted(rightsVersions);
+        // assert isBST(version);
+
+        // assert valuesVersions == old(valuesVersions);
+        // assert values == old(values);
+        // assert ValueSetAt(version) == OldValueSet + {value};
+        // assert RightAt(version) == res;
+        // assert LeftAt(version) == old(LeftAt(version));
+        assert ValueSetUnions(version)
+         by {
+          assert Sorted(old(valuesVersions));
+          assert Sorted(old(ValueSetsVersions));
+          assert |old(ValueSetsVersions)| == |old(ValueSets)|;
+          assert |old(valuesVersions)| == |old(values)|;
+          assert |old(ValueSetsVersions)| > 0;
+          assert |old(valuesVersions)| > 0;
+
+          assert ValueSetsVersions == old(ValueSetsVersions) + [version];
+          assert ValueSetAt(version) == old(ValueSetAt(version)) + {value};
+          assert old(ValueSetAt(version)) == ValueSets[|ValueSets| - 2];
+          assert old(ValueAt(version)) == ValueAt(version);
+          assert old(ValueAt(version)) in  old(ValueSetAt(version));
+          assert old(LeftValueSetAt(version)) < old(ValueSetAt(version));
+          assert old(RightValueSetAt(version)) < old(ValueSetAt(version));
+
+          assert ValueSetAt(version) == old(ValueSetAt(version)) + {value};
+          assert ValueAt(version) == old(ValueAt(version));
+          assert LeftValueSetAt(version) == old(LeftValueSetAt(version));
+          assert old(RightAt(version)) == null;
+          assert old(RightValueSetAt(version)) == {};
+          assert RightAt(version) == res;
+          assert RightValueSetAt(version) == {value};
+          assert old(ValueSetAt(version)) == {old(ValueAt(version))} + old(LeftValueSetAt(version)) + old(RightValueSetAt(version));
+        }
+      } else {
+        assume false;
+        res := right.Insert(version, value);
+        if (res != null) {
+          assert Sorted(rightsVersions);
+          Repr := Repr + {res};
+          ValueSets := ValueSets + [ValueSet() + {value}];
+          ValueSetsVersions := ValueSetsVersions + [version];
+          assert Sorted(ValueSetsVersions);
+          assert valuesVersions == old(valuesVersions);
+          assert values == old(values);
+        }
+      }
+    } else {
+      res := null;
+
+      assert ValueSetsVersions == old(ValueSetsVersions);
+      assert rightsVersions == old(rightsVersions);
+      assert leftsVersions == old(leftsVersions);
+      assert ValueSets == old(ValueSets);
+      assert rights == old(rights);
+      assert lefts == old(lefts);
+    }
+
+    assert valuesVersions == old(valuesVersions);
+    assert values == old(values);
+  }
 }
